Update interop_printer for better error reporting + Aes accordingly

src/arch/x64/interop/Aes.fst
@@ -27,7 +27,6 @@ assume val addrs: addr_map
 // TODO: Complete with your pre- and post-conditions
 let pre_cond (h:HS.mem) (input_key:B.buffer UInt8.t) (output_key:B.buffer UInt8.t) = live h input_key /\ live h output_key /\ disjoint input_key output_key /\ length input_key % 16 == 0 /\ length output_key % 16 == 0 /\
   length input_key == 16 /\ length output_key == 176
-
 let post_cond (h0:HS.mem) (h1:HS.mem) (input_key:B.buffer UInt8.t) (output_key:B.buffer UInt8.t) = live h0 input_key /\ live h0 output_key /\ live h1 input_key /\ live h1 output_key /\ length input_key % 16 == 0 /\ length output_key % 16 == 0 /\   
 length input_key == 16 /\ length output_key == 176 /\
 M.modifies (M.loc_buffer output_key) h0 h1 /\
@@ -40,11 +39,42 @@ M.modifies (M.loc_buffer output_key) h0 h1 /\
   (forall j. 0 <= j /\ j <= 10 ==>
     Seq.index (BV.as_seq h1 output_b) j ==
     Seq.index result j))
-     
 
 //The initial registers and xmms
 assume val init_regs:reg -> nat64
 assume val init_xmms:xmm -> quad32
+
+#set-options "--initial_fuel 4 --max_fuel 4 --initial_ifuel 2 --max_ifuel 2"
+// TODO: Prove these two lemmas if they are not proven automatically
+let implies_pre (h0:HS.mem) (input_key:B.buffer UInt8.t) (output_key:B.buffer UInt8.t) : Lemma
+  (requires pre_cond h0 input_key output_key )
+  (ensures (
+  let buffers = input_key::output_key::[] in
+  let (mem:mem) = {addrs = addrs; ptrs = buffers; hs = h0} in
+  let addr_input_key = addrs input_key in
+  let addr_output_key = addrs output_key in
+  let regs = fun r -> begin match r with
+    | Rdi -> addr_input_key
+    | Rsi -> addr_output_key
+    | _ -> init_regs r end in
+  let xmms = init_xmms in
+  let s0 = {ok = true; regs = regs; xmms = xmms; flags = 0; mem = mem} in
+  length_t_eq (TBase TUInt128) input_key;
+  length_t_eq (TBase TUInt128) output_key;
+  va_pre (va_code_aes ()) s0 input_key output_key )) =
+  length_t_eq (TBase TUInt128) input_key;
+  length_t_eq (TBase TUInt128) output_key;
+  ()
+
+let implies_post (va_s0:va_state) (va_sM:va_state) (va_fM:va_fuel) (input_key:B.buffer UInt8.t) (output_key:B.buffer UInt8.t)  : Lemma
+  (requires pre_cond va_s0.mem.hs input_key output_key /\
+    va_post (va_code_aes ()) va_s0 va_sM va_fM input_key output_key )
+  (ensures post_cond va_s0.mem.hs va_sM.mem.hs input_key output_key ) =
+  length_t_eq (TBase TUInt128) input_key;
+  length_t_eq (TBase TUInt128) output_key;
+  assert (forall j. 0 <= j /\ j <= 10 ==>
+    Seq.index (BV.as_seq va_sM.mem.hs (BV.mk_buffer_view output_key Views.view128)) j == buffer128_read output_key j va_sM.mem);    
+  ()
 
 val aes: input_key:B.buffer UInt8.t -> output_key:B.buffer UInt8.t -> ST unit
 	(requires (fun h -> pre_cond h input_key output_key ))
@@ -52,7 +82,6 @@ val aes: input_key:B.buffer UInt8.t -> output_key:B.buffer UInt8.t -> ST unit
 
 val ghost_aes: input_key:B.buffer UInt8.t -> output_key:B.buffer UInt8.t -> (h0:HS.mem{pre_cond h0 input_key output_key }) -> GTot (h1:HS.mem{post_cond h0 h1 input_key output_key })
 
-#set-options "--initial_fuel 4 --max_fuel 4 --initial_ifuel 2 --max_ifuel 2"
 let ghost_aes input_key output_key h0 =
   let buffers = input_key::output_key::[] in
   let (mem:mem) = {addrs = addrs; ptrs = buffers; hs = h0} in
@@ -66,6 +95,7 @@ let ghost_aes input_key output_key h0 =
   let s0 = {ok = true; regs = regs; xmms = xmms; flags = 0; mem = mem} in
   length_t_eq (TBase TUInt128) input_key;
   length_t_eq (TBase TUInt128) output_key;
+  implies_pre h0 input_key output_key ;
   let s1, f1 = va_lemma_aes (va_code_aes ()) s0 input_key output_key  in
   // Ensures that the Vale execution was correct
   assert(s1.ok);
@@ -78,9 +108,7 @@ let ghost_aes input_key output_key h0 =
   assert(s0.regs R15 == s1.regs R15);
   // Ensures that va_code_aes is actually Vale code, and that s1 is the result of executing this code
   assert (va_ensure_total (va_code_aes ()) s0 s1 f1);
-  // This assertion is manually added
-  assert (forall j. 0 <= j /\ j <= 10 ==>
-    Seq.index (BV.as_seq s1.mem.hs (BV.mk_buffer_view output_key Views.view128)) j == buffer128_read output_key j s1.mem);  
+  implies_post s0 s1 f1 input_key output_key ;
   s1.mem.hs
 
 let aes input_key output_key  =
